extraction/examples/ElmExtractTests.v
@@ -1,0 +1,120 @@
+(** * Tests for extraction to Elm *)
+(** Uses the same pretty-printer as Midlang, since Midlang is a fork of Elm.
+    The examples are writen into files which are later processed and passed to the Elm compiler as part of the building process. *)
+
+(** Warning: this file does not work in the interactive mode due to the problems with paths for [Redirect]. We have to stick to the path, relative to the project root and in the interactive mode current directory is different. *)
+From ConCert.Extraction Require Import Common.
+From ConCert.Extraction Require Import MidlangExtract.
+From ConCert.Extraction Require Import Optimize.
+From ConCert.Extraction Require Import PrettyPrinterMonad.
+From ConCert.Extraction Require Import ResultMonad.
+From ConCert.Extraction Require Import MidlangExtractTests.
+From Coq Require Import Arith.
+From Coq Require Import String.
+From Coq Require Import String Ascii.
+From Coq Require Import List.
+From MetaCoq.Template Require Import Ast.
+From MetaCoq.Template Require Import Loader.
+From MetaCoq.Template Require Import TemplateMonad.
+From MetaCoq Require Import monad_utils.
+From MetaCoq Require Import utils.
+
+Import MonadNotation.
+
+Definition wrapped (p : program) (pre post : string) : result string string :=
+  entry <- match p.2 with
+           | tConst kn _ => ret kn
+           | _ => Err "Expected program to be a tConst"
+           end;;
+  Σ <- specialize_erase_debox_template_env p.1 [entry] [];;
+  '(_, s) <- finish_print (print_env Σ p.1 (fun _ => None));;
+  ret (pre ++ nl ++ s ++ nl ++ post).
+
+Module ElmExamples.
+  Definition Preambule mod_name :=
+    String.concat nl
+                  ["module " ++ mod_name ++ " exposing (..)";
+                  "import Test";
+                  "import Html";
+                  "import Expect exposing (Expectation)"].
+
+  Definition main_and_test (test : string) :=
+    "main = Html.text "++ parens false ("Debug.toString " ++ parens false test) ++ nl ++
+    "suite = Test.test (Debug.toString 1)" ++ parens false ("\ _ -> " ++ test).
+
+  MetaCoq Quote Recursively Definition map_syn := List.map.
+  Definition result_map :=
+    String.concat nl
+      ["type List a";
+      "  = Nil";
+      "  | Cons a (List a)";
+        "";
+      "map : (a -> b) -> List a -> List b";
+      "map f =";
+      "  let";
+      "    map2 l =";
+      "      case l of";
+      "        Nil ->";
+      "          Nil";
+      "        Cons a t ->";
+      "          Cons (f a) (map2 t)";
+      "  in";
+      "  map2"].
+
+
+  Redirect "./extraction/examples/elm-extract/Map.elm" Compute wrapped map_syn
+          (Preambule "Map")
+          (main_and_test "Expect.equal (map (\x->x+1) (Cons 1 (Cons 0 Nil))) (Cons 2 (Cons 1 Nil))").
+
+  Example ElmList_map :
+    extract map_syn = Ok result_map.
+  Proof. reflexivity. Qed.
+
+  MetaCoq Quote Recursively Definition foldl_syn := List.fold_left.
+  Definition result_foldl :=
+    String.concat nl
+      ["type List a";
+      "  = Nil";
+      "  | Cons a (List a)";
+        "";
+      "fold_left : (a -> b -> a) -> List b -> a -> a";
+      "fold_left f =";
+        "  let";
+      "    fold_left2 l a0 =";
+      "      case l of";
+      "        Nil ->";
+      "          a0";
+      "        Cons b t ->";
+      "          fold_left2 t (f a0 b)";
+      "  in";
+      "  fold_left2"].
+
+  Redirect "./extraction/examples/elm-extract/Fold.elm" Compute wrapped foldl_syn
+         (Preambule "Fold")
+         (main_and_test "(Expect.equal (fold_left (+) (Cons 1 (Cons 0 Nil)) 0)) 1").
+
+  Example ElmList_foldl :
+    extract foldl_syn = Ok result_foldl.
+  Proof. reflexivity. Qed.
+
+  Import Lia.
+
+  Program Definition inc_counter (st : nat) (inc : {z : nat | 0 <? z}) :
+    {new_st : nat | st <? new_st} :=
+    st + inc.
+  Next Obligation.
+    intros st inc. unfold is_true in *.
+    destruct inc;simpl.
+    rewrite NPeano.Nat.ltb_lt in *. lia.
+  Qed.
+
+  MetaCoq Run (t <- tmQuoteRecTransp inc_counter false ;;
+               tmDefinition "inc_counter_syn" t).
+
+  Redirect "./extraction/examples/elm-extract/Increment.elm"
+  Compute wrapped inc_counter_syn
+         (Preambule "Increment")
+         (main_and_test "Expect.equal (inc_counter O (Exist (S O))) (Exist (S O))").
+
+
+End ElmExamples.
