extraction/examples/ForPaper.v
@@ -1,7 +1,7 @@
 From Coq Require Import PeanoNat ZArith Notations Bool.
 
 From MetaCoq.Template Require Import Loader.
-From MetaCoq.Erasure Require Import SafeTemplateErasure Debox.
+From MetaCoq.Erasure Require Import SafeTemplateErasure Loader.
 From MetaCoq.Erasure Require ErasureFunction.
 From MetaCoq.Erasure Require SafeErasureFunction.
 From MetaCoq.Template Require Import config.
@@ -11,7 +11,7 @@ From MetaCoq.PCUIC Require Import PCUICAst PCUICAstUtils PCUICTyping
      TemplateToPCUIC.
 
 From ConCert.Embedding Require Import MyEnv.
-From ConCert.Extraction Require Import LiquidityExtract LPretty.
+From ConCert.Extraction Require Import LiquidityExtract LPretty Common.
 
 From Coq Require Import List String.
 
@@ -22,6 +22,42 @@ Import MonadNotation.
 
 Open Scope nat.
 
+Definition rank2_ex : forall (A : Type), A -> (forall A : Type, A -> A) -> A :=
+fun A a f => f _ a.
+Extraction rank2_ex.
+
+(** Cumulativity *)
+Definition const_zero {A : Type} (a : A) := 0.
+
+Definition const_zero_app_prop := const_zero True.
+Definition const_zero_app_type := const_zero 0.
+
+MetaCoq Erase (unfolded const_zero_app_prop).
+MetaCoq Erase (unfolded const_zero_app_type).
+
+Definition weird_map {A B} (f : A -> B) (l : list A) : unit -> list B :=
+  let g := @map A in
+  fun _ : unit => g B f l.
+
+MetaCoq Erase (unfolded @weird_map).
+
+Definition ex_prop (n : nat) (p : (0 < n)%nat) := n.
+
+(** Let's return something more tricky that could not be optimised easily *)
+Definition ex3 (n : nat) (b : bool) :=
+  let f := match b with | true => ex_prop (S n) | false => fun _ => 0 end in
+  fun _ : unit => f (Nat.lt_0_succ n) + f (Nat.lt_0_succ n).
+
+MetaCoq Erase (unfolded ex3).
+Extraction ex3.
+
+Definition ex4 (n : nat) (b : bool) :=
+  (match b with
+  | true => (fun (p : 0 < S n) => n)
+  | false => fun _ => 0
+  end) (Nat.lt_0_succ n).
+
+MetaCoq Erase (unfolded ex4).
 
 Definition erase_print_with_boxes (p : Ast.program) : string :=
   let p := fix_program_universes p in
